sorry removed, restructuring to Optics

C11-BackEnds/Clean/src/Clean.thy
@@ -36,13 +36,13 @@
 
 (*
  * Clean --- a basic abstract ("shallow") programming language for test and proof.
- * Burkhart Wolff, Frédéric Tuong and Chantal Keller, LRI, Univ. Paris-Saclay, France
+ * Burkhart Wolff and Frédéric Tuong, LRI, Univ. Paris-Saclay, France
  *)
 
 chapter \<open>The Clean Language\<close>
 
 theory Clean
-  imports Lens_Laws Symbex_MonadSE
+  imports Optics Symbex_MonadSE
   keywords "global_vars" "local_vars_test" :: thy_decl 
      and "returns" "pre" "post" "local_vars" "variant" 
      and "function_spec" :: thy_decl
@@ -137,9 +137,8 @@ record  control_state =
             break_status  :: bool
             return_status :: bool
 
-ML\<open>
-val t = @{term "\<sigma> \<lparr> break_status := False \<rparr>"}
-\<close>
+(* ML level representation: *)
+ML\<open> val t = @{term "\<sigma> \<lparr> break_status := False \<rparr>"}\<close>
 
 (* break quits innermost while or for, return quits an entire execution sequence. *)  
 definition break :: "(unit, ('\<sigma>_ext) control_state_ext) MON\<^sub>S\<^sub>E"
@@ -184,33 +183,6 @@ text\<open> On the basis of the control-state, assignments, conditionals and loo
 text\<open>For Reasoning over Clean programs, we need the notion of independance of an
      update from the control-block: \<close>
 
-find_theorems  "control_state.break_status_update"
-
-
-fun      upd_hd :: "('a \<Rightarrow> 'a) \<Rightarrow> 'a list \<Rightarrow> 'a list" 
-  where "upd_hd f [] = []"
-      | "upd_hd f (a#S) = f a # S"
-
-lemma tl_map_hd [simp] :"tl (upd_hd f S) = tl S" 
-  by (metis list.sel(3) upd_hd.elims)
-
-
-definition upd2put :: "(('d \<Rightarrow> 'b) \<Rightarrow> 'a \<Rightarrow> 'c) \<Rightarrow> 'a \<Rightarrow> 'b \<Rightarrow> 'c"
-  where   "upd2put f = (\<lambda>\<sigma>. \<lambda> b. f (\<lambda>_. b) \<sigma>)"
-
-definition create\<^sub>L 
-  where "create\<^sub>L getv updv = \<lparr>lens_get = getv,lens_put = upd2put updv\<rparr>"
-
-definition "hd\<^sub>L = create\<^sub>L hd upd_hd"   (* partial lenses needed  ?*)
-
-definition "map_nth i = (\<lambda>f l. list_update l i (f (l ! i)))"
-
-lemma indep_list_lift : 
-     "X \<bowtie> create\<^sub>L getv updv 
-      \<Longrightarrow> (\<lambda>f \<sigma>. updv (\<lambda>_. f (getv \<sigma>)) \<sigma>) = updv 
-      \<Longrightarrow> X \<bowtie> create\<^sub>L (hd \<circ> getv ) (updv \<circ> upd_hd)"
-  unfolding create\<^sub>L_def o_def Lens_Laws.lens_indep_def upd2put_def
-  by (auto,metis (no_types)) (metis (no_types))
 
 definition break_status\<^sub>L 
   where "break_status\<^sub>L = create\<^sub>L control_state.break_status control_state.break_status_update"
@@ -254,6 +226,8 @@ lemma strong_vs_weak_upd :
   by(drule strong_vs_weak_ci, auto)
 
 
+text\<open>This quite tricky proof establishes the face that the special case 
+     \<open>hd(getv \<sigma>) = []\<close> for \<open>getv \<sigma> = []\<close> is finally irrelevant in our setting.\<close>
 lemma strong_vs_weak_upd_list : 
   assumes * :  "\<sharp>! (create\<^sub>L (getv:: 'b control_state_scheme \<Rightarrow> 'c list) 
                             (updv:: ('c list \<Rightarrow> 'c list) \<Rightarrow> 'b control_state_scheme \<Rightarrow> 'b control_state_scheme))"  
@@ -262,46 +236,31 @@ lemma strong_vs_weak_upd_list :
   shows        "\<sharp> (updv \<circ> upd_hd)"
 proof - 
   have *** : "\<sharp>! (create\<^sub>L (hd \<circ> getv ) (updv \<circ> upd_hd))"
-    using * ** by (simp add: indep_list_lift strong_control_independence_def)
+       using * ** by (simp add: indep_list_lift strong_control_independence_def)
   show "\<sharp> (updv \<circ> upd_hd)"
     apply(rule strong_vs_weak_upd)
      apply(rule ***)
-    apply(rule ext, rule ext)
-    sorry
+    apply(rule ext, rule ext, simp)
+    apply(subst (2) **[symmetric])
+  proof -
+    fix f:: "'c \<Rightarrow> 'c" fix \<sigma> :: "'b control_state_scheme"
+    show "updv (upd_hd (\<lambda>_. f (hd (getv \<sigma>)))) \<sigma> = updv (\<lambda>_. upd_hd f (getv \<sigma>)) \<sigma>"
+      proof (cases "getv \<sigma>")
+        case Nil
+        then show ?thesis           
+          by (simp,metis (no_types) "**" upd_hd.simps(1))
+      next
+        case (Cons a list)
+        then show ?thesis 
+        proof -
+          have "(\<lambda>c. f (hd (getv \<sigma>))) = ((\<lambda>c. f a)::'c \<Rightarrow> 'c)"
+            using local.Cons by auto
+          then show ?thesis
+            by (metis (no_types) "**" local.Cons upd_hd.simps(2))
+        qed
+      qed
+    qed
 qed
-thm list.sel(1) list.sel(3) list.simps(3) o_apply upd_hd.elims
-(* this does not seem hopeless:
-  sledgehammer offers two different proofs:
-
-  by (metis "**" list.sel(1) list.sel(3) list.simps(3) o_apply upd_hd.elims)
-
-  and
-
-proof -
-  fix f :: "'c \<Rightarrow> 'c" and \<sigma> :: "'b control_state_scheme"
-{ fix cc :: 'c
-  have "\<forall>f cs. esk1_3 f cs (upd_hd f cs) = (hd cs::'c) \<or> cs = []"
-    by (metis list.sel(1) upd_hd.elims) (* > 1.0 s, timed out *)
-  then have ff1: "\<forall>f cs. (hd cs::'c) # esk2_3 f cs (upd_hd f cs) = cs \<or> cs = []"
-by (metis upd_hd.elims) (* > 1.0 s, timed out *)
-have "\<forall>c cs f. upd_hd f ((c::'c) # cs) = f c # cs"
-  by simp
-  then have ff2: "\<forall>f cs. f (hd cs::'c) # tl cs = upd_hd f cs \<or> cs = []"
-    using ff1 by (metis list.sel(3))
-then have "\<forall>c ca. updv (\<lambda>cs. c # tl (getv ca)) ca = updv (upd_hd (\<lambda>ca. c)) ca \<or> getv ca = []"
-  by (metis (no_types) "**")
-  then have "\<forall>f c. updv (upd_hd (\<lambda>ca. f (hd (getv c)))) c = updv (upd_hd f) c \<or> getv c = []"
-    using ff2 
-    
-    by (metis "**") (* > 1.0 s, timed out *)
-then have "updv (upd_hd (\<lambda>c. f (hd (getv \<sigma>)))) \<sigma> = updv (upd_hd f) \<sigma>"
-by (metis (no_types) "**" list.simps(3) upd_hd.elims)
-then have "(updv \<circ> upd_hd) (\<lambda>c. f ((hd \<circ> getv) \<sigma>)) \<sigma> = (updv \<circ> upd_hd) f \<sigma> \<or> f ((hd \<circ> getv) \<sigma>) = f cc"
-by simp }
-  then show "(updv \<circ> upd_hd) (\<lambda>c. f ((hd \<circ> getv) \<sigma>)) \<sigma> = (updv \<circ> upd_hd) f \<sigma>"
-    by meson
-qed
-*)
 
 lemma exec_stop_vs_control_independence [simp]:
   "\<sharp> upd \<Longrightarrow> exec_stop (upd f \<sigma>) = exec_stop \<sigma>"
